Veir/IR/Buffed/RawReadWriteLemmas/Operations.lean
@@ -11,7 +11,7 @@ namespace Veir.Buffed
 
 section read_write
 
-variable [HasOpInfo OpInfo] [SerializableOpInfo OpInfo] [HasBuffedProperties OpInfo] {ctx : Sim.IRContext OpInfo}
+variable [HasOpInfo OpInfo] [SerializableOpInfo OpInfo] [HasBuffedOpCode OpInfo] {ctx : Sim.IRContext OpInfo}
 
 /-! ## OperationMPtr.readPrev! -/
 
